\documentclass[12pt]{article}
\usepackage{amsmath}
\usepackage{graphicx}
\usepackage{hyperref}
\usepackage[latin1]{inputenc}
\usepackage{listings}
\usepackage{pgfplots}
\usepackage{makecell}
\setlength{\tabcolsep}{6pt}
\renewcommand{\labelitemi}{$\textendash$}
\renewcommand{\arraystretch}{2.0}
\newcommand\aug{\fboxsep=-\fboxrule\!\!\!\fbox{\strut}\!\!\!}

\title{CS3081: Assignment 1}
\author{Conor McCauley - 17323203}
\date{February 26, 2020}

\begin{document}

\maketitle

\section*{Answers}

\subsection*{Question 2.31}

\noindent a. (ii) $13$

\noindent b. (i) $0$

\subsection*{Question 3.2}

\noindent a. (ii) $0.8125$

\noindent b. (ii) $0.85261$

\noindent c. (iv) $0.85261$

\subsection*{Question 4.24}

\noindent a. (i)

$$
\begin{pmatrix}
    -0.7143 & 0 & 1.4286 \\
    0.2571 & 0.1 & 0.2857 \\
    -0.2286 & -0.2 & 0.8571
\end{pmatrix}
$$

\noindent b. (i)

$$
\begin{pmatrix}
    1.6667 & 2.8889 & -2.2222 & 1 \\
    0 & 0.3333 & -0.3333 & 0 \\
    -0.3333 & -0.4444 & 0.1111 & 0 \\
    1.5 & 2 & -1.5 & 0.5
\end{pmatrix}
$$

\section*{Solutions}

\subsection*{Question 2.31}

\noindent a.

\begin{center}

$$ \det\begin{pmatrix} 1 & 5 & 4 \\ 2 & 3 & 6 \\ 1 & 1 & 1 \end{pmatrix} $$
$$
= 1 \cdot \begin{vmatrix} 3 & 6 \\ 1 & 1 \end{vmatrix}
- 5 \cdot \begin{vmatrix} 2 & 6 \\ 1 & 1 \end{vmatrix}
+ 4 \cdot \begin{vmatrix} 2 & 3 \\ 1 & 1 \end{vmatrix}
$$
$$ = 1 \cdot (3\cdot1 - 6\cdot1) - 5 \cdot (2\cdot1 - 6\cdot1) + 4 \cdot (2\cdot1 - 3\cdot1) $$
$$ = 1 \cdot (3 - 6) - 5 \cdot (2 - 6) + 4 \cdot (2 - 3) $$
$$ = 1 \cdot (-3) - 5 \cdot (-4) + 4 \cdot (-1) $$
$$ = -3 + 20 - 4 = 13 $$

\end{center}

\noindent b.

\begin{center}

$$ \det\begin{pmatrix} 1 & 2 & 3 & 4 \\ 5 & 6 & 7 & 8 \\ 9 & 10 & 11 & 12 \\ 13 & 14 & 15 & 16 \end{pmatrix} $$

$$
= 1 \cdot \begin{vmatrix} 6 & 7 & 8 \\ 10 & 11 & 12 \\ 14 & 15 & 16 \end{vmatrix}
- 2 \cdot \begin{vmatrix} 5 & 7 & 8 \\ 9 & 11 & 12 \\ 13 & 15 & 16 \end{vmatrix}
+ 3 \cdot \begin{vmatrix} 5 & 6 & 8 \\ 9 & 10 & 12 \\ 13 & 14 & 16 \end{vmatrix}
- 4 \cdot \begin{vmatrix} 5 & 6 & 7 \\ 9 & 10 & 11 \\ 13 & 14 & 15 \end{vmatrix}
$$

$$
= 1 \cdot \left(
6 \cdot \begin{vmatrix} 11 & 12 \\ 15 & 16 \end{vmatrix}
- 7 \cdot \begin{vmatrix} 10 & 12 \\ 14 & 16 \end{vmatrix} 
+ 8 \cdot \begin{vmatrix} 10 & 11 \\ 14 & 15 \end{vmatrix} 
\right)
$$
$$
- 2 \cdot \left(
5 \cdot \begin{vmatrix} 11 & 12 \\ 15 & 16 \end{vmatrix}
- 7 \cdot \begin{vmatrix} 9 & 12 \\ 13 & 16 \end{vmatrix} 
+ 8 \cdot \begin{vmatrix} 9 & 11 \\ 13 & 15 \end{vmatrix} 
\right)
$$
$$
+ 3 \cdot \left(
5 \cdot \begin{vmatrix} 10 & 12 \\ 14 & 16 \end{vmatrix}
- 6 \cdot \begin{vmatrix} 9 & 12 \\ 13 & 16 \end{vmatrix} 
+ 8 \cdot \begin{vmatrix} 9 & 10 \\ 13 & 14 \end{vmatrix} 
\right)
$$
$$
- 4 \cdot \left(
5 \cdot \begin{vmatrix} 10 & 11 \\ 14 & 15 \end{vmatrix}
- 6 \cdot \begin{vmatrix} 9 & 11 \\ 13 & 15 \end{vmatrix} 
+ 7 \cdot \begin{vmatrix} 9 & 10 \\ 13 & 14 \end{vmatrix} 
\right)
$$

$$
= 1 \cdot (
6 \cdot (11\cdot16 - 12\cdot15)
- 7 \cdot (10\cdot16 - 12\cdot14)
+ 8 \cdot (10\cdot15 - 11\cdot14)
)
$$
$$
- 2 \cdot (
5 \cdot (11\cdot16 - 12\cdot15)
- 7 \cdot (9\cdot16 - 12\cdot13)
+ 8 \cdot (9\cdot15 - 11\cdot13)
)
$$
$$
+ 3 \cdot (
5 \cdot (10\cdot16 - 12\cdot14)
- 6 \cdot (9\cdot16 - 12\cdot13)
+ 8 \cdot (9\cdot14 - 10\cdot13)
)
$$
$$
- 4 \cdot (
5 \cdot (10\cdot15 - 11\cdot14)
- 6 \cdot (9\cdot15 - 11\cdot13)
+ 7 \cdot (9\cdot14 - 10\cdot13)
)
$$

$$
= 1 \cdot (
6 \cdot (176 - 180)
- 7 \cdot (160 - 168)
+ 8 \cdot (150 - 154)
)
$$
$$
- 2 \cdot (
5 \cdot (176 - 180)
- 7 \cdot (144 - 156)
+ 8 \cdot (135 - 143)
)
$$
$$
+ 3 \cdot (
5 \cdot (160 - 168)
- 6 \cdot (144 - 156)
+ 8 \cdot (126 - 130)
)
$$
$$
- 4 \cdot (
5 \cdot (150 - 154)
- 6 \cdot (135 - 143)
+ 7 \cdot (126 - 130)
)
$$

$$ = 1 \cdot (6 \cdot (-4) - 7 \cdot (-8) + 8 \cdot (-4)) $$
$$ - 2 \cdot (5 \cdot (-4) - 7 \cdot (-12) + 8 \cdot (-8)) $$
$$ + 3 \cdot (5 \cdot (-8) - 6 \cdot (-12) + 8 \cdot (-4)) $$
$$ - 4 \cdot (5 \cdot (-4) - 6 \cdot (-8) + 7 \cdot (-4)) $$

$$ = 1 \cdot (-24 + 56 - 32) - 2 \cdot (-20 + 84 - 64) $$
$$ + 3 \cdot (-40 + 72 - 32) - 4 \cdot (-20 + 48 - 28) $$

$$ = 1 \cdot 0 - 2 \cdot 0 + 3 \cdot 0 - 4 \cdot 0 = 0 $$

\end{center}

\subsection*{Question 3.1}

\noindent a.

\begin{center}
    \begin{tabular}{|c||c|c|c|c|c|c|}
        \hline
        & $a$ & $b$ & $c$ & $f(a)$ & $f(c)$ & Comment \\
        \hline
        $0$ & $0$ & $1$ & $\frac{0+1}{2} = 0.5$ & $-2$ & $-0.713$ & \makecell{$f(a)$ and $f(c)$ have same sign\\so set $a=c$} \\
        $1$ & $0.5$ & $1$ & $\frac{0.5+1}{2} = 0.75$ & $-0.713$ & $-0.1947$ & \makecell{$f(a)$ and $f(c)$ have same sign\\so set $a=c$} \\
        $2$ & $0.75$ & $1$ & $\frac{0.75+1}{2} = 0.875$ & $-0.1947$ & $0.0412$ & \makecell{$f(a)$ and $f(c)$ have different\\sign so set $b=c$} \\
        $3$ & $0.75$ & $0.875$ & $\frac{0.75+0.875}{2} = 0.8125$ & $-0.1947$ & $-0.0749$ & $root = 0.8125$ \\
        \hline
    \end{tabular}
\end{center}

\noindent b.

\begin{center}
    \begin{tabular}{|c||c|c|c|}
        \hline
        $n$ & $x_{n-1}$ & $x_{n}$ & $x_{n+1}$ \\
        \hline
        $2$ & $x_{1} = 0$ & $x_{2} = 1$ &
        $ x_{3} = 1 - \frac{f(1) \cdot (0 - 1)}{f(0) - f(1)} = 1 - \frac{0.264 \cdot -1}{{-2} - 0.264} = 0.883 $ \\
        $3$ & $x_{2} = 1$ & $ x_{3} = 0.883$ & $x_{4} = 0.883 - \frac{f(0.883) \cdot (1 - 0.883)}{f(1) - f(0.883)} = 0.883 - \frac{0.056 \cdot 0.117}{0.264 - 0.056} = 0.8515 $ \\
        $4$ & $x_{3} = 0.883$ & $x_{4} = 0.8515$ & \makecell{$ x_{5} = 0.8515 - \frac{f(0.8515) \cdot (0.883 - 0.8515)}{f(0.883) - f(0.8515)} = 0.8515 - \frac{-0.002 \cdot 0.0315}{0.056 - (-0.002)} $\\$ = 0.852 \approx 0.85261 $} \\
        \hline
    \end{tabular}
\end{center}

\noindent c. In order to use Newton's method we must first find the derivative of $f(x)$:

$$ \frac{d}{dx} (x - 2e^{-x}) $$
$$ = 1 - \frac{d}{dx} (2e^{-x}) $$
$$ = 1 - (-1 \cdot 2e^{-x}) $$
$$ = 1 + 2e^{-x} $$

\begin{center}
    \begin{tabular}{|c||c|c|}
        \hline
        $n$ & $x_{n}$ & $x_{n+1}$ \\
        \hline
        $1$ & $1$ & $ 1 - \frac{1 - 2e^{-1}}{1 + 2e^{-1}} = 0.84776 $ \\
        \hline
        $2$ & $0.84776$ & $ 0.84776 - \frac{0.84776 - 2e^{-0.84776}}{1 + 2e^{-0.84776}} = 0.8526 $ \\
        \hline
        $3$ & $0.8526$ & $ 0.8526 - \frac{0.8526 - 2e^{-0.8526}}{1 + 2e^{-0.8526}} = 0.852606 \approx 0.85261 $ \\
        \hline
    \end{tabular}
\end{center}

\subsection*{Question 4.24}

\noindent The following Matlab code can be used to calculate the inverse of the matrices given in the question:

\begin{lstlisting}[language=Matlab]
    % calculate the inverse of a matrix A
    function [Ainv] = Inverse(A)
        
        [N, ~] = size(A);   % get the size of the matrix
        Ainv = Identity(N); % construct the identity matrix
        
        % for each row in the (augmented) matrix
        for i = 1:N
            
            % make diagonal column 1
            u = A(i, i);
            for j = 1:N
                A(i, j) = A(i, j) / u;
                Ainv(i, j) = Ainv(i, j) / u;
            end
            
            % make non-diagonal columns 0
            for j = 1:N
                if j ~= i
                    v = A(j, i);
                    for k = 1:N
                        A(j, k) = A(j, k) - (A(i, k) * v);
                        Ainv(j, k) = Ainv(j, k) - (Ainv(i, k) * v);
                    end
                end
            end
            
        end
        
    end
    
    % return the identity matrix of size N
    function [Imat] = Identity(N)
        Imat = zeros(N, N);
        for i = 1:N
            Imat(i, i) = 1;
        end
    end
\end{lstlisting}

\noindent For the matrix in question (a) the code gives the following answer:

$$
\begin{pmatrix}
    -0.7143 & 0 & 1.4286 \\
    0.2571 & 0.1 & 0.2857 \\
    -0.2286 & -0.2 & 0.8571
\end{pmatrix}
$$

\noindent For the matrix in question (b) the code gives the following answer:

$$
\begin{pmatrix}
    1.6667 & 2.8889 & -2.2222 & 1 \\
    0 & 0.3333 & -0.3333 & 0 \\
    -0.3333 & -0.4444 & 0.1111 & 0 \\
    1.5 & 2 & -1.5 & 0.5
\end{pmatrix}
$$

\noindent These results both match the answers given in (i).

\end{document}
